\documentclass{amsart}

\input{StandardPaper2.tex}
\input{local_definitions.tex}

\title[]{CMC surfaces with free boundary on the sphere}

\curraddr{}
\email{}

\dedicatory{}
\subjclass[2010]{}
\keywords{}

\begin{document}

\begin{abstract}
\end{abstract}

\maketitle

\section{The set up}

Let \(M^n \subseteq \R^{n+1}\) be a smooth, oriented \(n\)-dimensional hypersurface with boundary \(\partial M\) lying on the unit sphere \(\S^n = \{\|x\| = 1\}\). Let \(\nor\) denote the unit normal to \(M\), \(H\) the mean curvature of \(M\) with respect to \(\nor\) and \(\norS\) the unit normal to the sphere \(\S^n\). Also let \(s = \inpr{X}{\nor}\) denote the support function of \(M\).

We assume that,
\begin{enumerate}
\item \(H \equiv \text{const}\) (CMC),
\item \(\inpr{\nor}{\norS} = 0\) along \(\partial M\) (\(M\) meets \(\S^n\) orthogonally),
\item \(s = \inpr{\nor}{X} > 0\) where \(X(x) = x\) is the position vector field on \(\R^{n+1}\) (\(M\) is star-shaped).
\end{enumerate}  
Note that \(\norS = X\) along \(\S^n\) and so we also have
\begin{enumerate}[resume]
\item \(s = \inpr{\nor}{X} = \inpr{\nor}{\norS} = 0 \text{ along } \partial M\) (zero boundary condition).
\end{enumerate}
The orthogonalality condition \(\inpr{\nor}{\norS} = 0\) implies that
\begin{enumerate}[resume]
\item \(\norS\) is tangent to \(M\) along \(\partial M\).
\end{enumerate}
Furthermore, since \(\partial M \subseteq \S^n\), we have \(T\partial M \subseteq TS^n\) along \(\partial M\) and hence \(T\partial M \perp N_{\S^n}\). We also have \(T\partial M \subseteq TM\) along \(\partial M\) and so \(T\partial M \perp N\). These two facts combined imply that
\begin{enumerate}[resume]
\item \(N_{\partial M} = N_{\S^n}\) along \(\partial M\).
\end{enumerate}

\section{Conventions}

We define the second fundamental form, \(h\) by
\[
D_X Y = \nabla_X Y - h(X, Y) N
\]
or in other words,
\[
h(X, Y) = -\inpr{D_X Y}{N} = \inpr{Y}{D_X N}.
\]

\section{The computation}

We use the following:
\begin{align}
\Delta |X|^2 &= -2 H s + 2n, \label{eq:DeltaX2} \\
\Delta s &= H - |A|^2 s. \label{eq:Deltas}
\end{align}

Integrating equation \eqref{eq:DeltaX2} gives
\[
\int_{\partial M} \inpr{X}{\nabla_{\norS} X} = \frac{1}{2} \int_M \Delta |X|^2 = -H \int_M s + n |M|.
\]
Observe that \(\nabla X = \Id\) and as noted, along \(\partial M\), \(X = \nor\) hence \(\inpr{X}{\nabla_{\norS} X} = \inpr{\norS}{\norS} = 1\). Therefore, \(|\partial M| = -H \int_M s + n |M|\) which we write as
\begin{equation}
\label{eq:intDeltaX2}
n |M| = H \int_M s + |\partial M|.
\end{equation}

Integrating equation \eqref{eq:Deltas} gives
\[
\begin{split}
H |M| - \int_M |A|^2 s &= \int \Delta s = \int_{\partial M} \nabla_{\norS} s \\
&= \int_{\partial M} \nabla_{\norS} \inpr{X}{\nor} = \int_{\partial_M} \inpr{\norS}{\nor} + \inpr{X}{\nabla_{\norS} \nor} \\
&= \int_{\partial_M} A(\norS, \norS).
\end{split}
\]
That is,
\begin{equation}
\label{eq:intDeltas}
H |M| = \int_M |A|^2 s + \int_{\partial M} A(\norS, \norS).
\end{equation}

Then from equations \eqref{eq:intDeltaX2} and \eqref{eq:intDeltas} we deduce
\[
H^2 \int_M s + H |\partial M| = n H |M| = n \int_M |A|^2 s + n \int_{\partial M} A(\norS, \norS).
\]
That is
\[
\int_{\partial_M} H - n A(\norS, \norS) = \int_M (n|A|^2 - H^2) s
\]
Notice that the term \(n|A|^2 - H^2 \geq 0\) equalling \(0\) precisely at umbilic points and that the star shaped assumption is \(s > 0\).

\end{document}
